Velvet2/Partial.lean
@@ -1,0 +1,2 @@
+import Velvet2.Partial.Defs
+import Velvet2.Partial.Instances
